define sound expression and update definition of typing

dsn/Lang/Dynamic/FinTyping.lean
@@ -4,13 +4,14 @@ import Lang.Dynamic.Transition
 import Lang.Dynamic.TransitionStar
 import Lang.Dynamic.Convergent
 import Lang.Dynamic.Divergent
+import Lang.Dynamic.Sound
 
 set_option pp.fieldNotation false
 
 namespace Lang.Dynamic
 
 def FinTyping (e : Expr) : Typ → Prop
-| .top => Convergent e ∨ Divergent e
+| .top => Sound e
 | .iso l body => FinTyping (.extract e l) body
 | .entry l body => FinTyping (.project e l) body
 | .path left right => ∀ e' , FinTyping e' left → FinTyping (.app e e') right
@@ -35,13 +36,7 @@ mutual
   | top =>
     unfold FinTyping
     intro h0
-    cases h0 with
-    | inl h2 =>
-      apply Or.inl
-      exact Convergent.subject_reduction transition h2
-    | inr h2 =>
-      apply Or.inr
-      exact Divergent.subject_reduction transition h2
+    exact Sound.subject_reduction transition h0
 
   | iso label body =>
     unfold FinTyping
@@ -117,13 +112,7 @@ mutual
   | top =>
     unfold FinTyping
     intro h0
-    cases h0 with
-    | inl h2 =>
-      apply Or.inl
-      exact Convergent.subject_expansion transition h2
-    | inr h2 =>
-      apply Or.inr
-      exact Divergent.subject_expansion transition h2
+    exact Sound.subject_expansion transition h0
 
   | iso label body =>
     unfold FinTyping
@@ -232,9 +221,9 @@ theorem FinTyping.path_determines_function
 : ∃ f , TransitionStar e (.function f)
 := by sorry
 
-theorem FinTyping.convergent_or_divergent
+theorem FinTyping.soundness
   (typing : FinTyping e t)
-: Convergent e ∨ Divergent e
+: Sound e
 := by cases t with
 | bot =>
   unfold FinTyping at typing
@@ -246,38 +235,23 @@ theorem FinTyping.convergent_or_divergent
 
 | iso label body =>
   unfold FinTyping at typing
-  have ih := FinTyping.convergent_or_divergent typing
-  cases ih with
-  | inl h =>
-    apply Or.inl
-    apply Convergent.evalcon_reflection
-    { apply EvalCon.extract label .hole }
-    { exact h }
-  | inr h =>
-    apply Or.inr
-    apply Divergent.evalcon_reflection
-    { apply EvalCon.extract label .hole }
-    { exact h }
+  have ih := FinTyping.soundness typing
+  apply Sound.evalcon_reflection
+  { apply EvalCon.extract label .hole }
+  { exact ih }
 
 | entry label body =>
   unfold FinTyping at typing
-  have ih := FinTyping.convergent_or_divergent typing
-  cases ih with
-  | inl h =>
-    apply Or.inl
-    apply Convergent.evalcon_reflection
-    { apply EvalCon.project label .hole }
-    { exact h }
-  | inr h =>
-    apply Or.inr
-    apply Divergent.evalcon_reflection
-    { apply EvalCon.project label .hole }
-    { exact h }
+  have ih := FinTyping.soundness typing
+  apply Sound.evalcon_reflection
+  { apply EvalCon.project label .hole }
+  { exact ih }
+
 
 | path left right =>
   apply FinTyping.path_determines_function at typing
   have ⟨f, h0⟩ := typing
-  apply Or.inl
+  apply Sound.convergent
   unfold Convergent
   exists (.function f)
 
@@ -286,19 +260,19 @@ theorem FinTyping.convergent_or_divergent
   unfold FinTyping at typing
   cases typing with
   | inl h =>
-    apply FinTyping.convergent_or_divergent h
+    apply FinTyping.soundness h
   | inr h =>
-    apply FinTyping.convergent_or_divergent h
+    apply FinTyping.soundness h
 
 | inter left right =>
   unfold FinTyping at typing
   have ⟨h0,h1⟩ := typing
-  apply FinTyping.convergent_or_divergent h0
+  apply FinTyping.soundness h0
 
 | diff left right =>
   unfold FinTyping at typing
   have ⟨h0,h1⟩ := typing
-  apply FinTyping.convergent_or_divergent h0
+  apply FinTyping.soundness h0
 | _ =>
   unfold FinTyping at typing
   exact False.elim typing
